Iterator/UnivLE.lean
@@ -1,0 +1,35 @@
+/-
+Copyright (c) 2025 Lean FRO, LLC. All rights reserved.
+Released under Apache 2.0 license as described in the file LICENSE.
+Authors: Paul Reichert
+-/
+prelude
+import Init.Core
+
+class UnivLE.{u, v} where
+  Lift : Type u → Type v
+  up : ∀ {α}, α → Lift α
+  down : ∀ {α}, Lift α → α
+  up_down : ∀ {α : Type u} {a : Lift α}, up (down a) = a
+  down_up : ∀ {α : Type u} {a : α}, down (up a) = a
+
+instance UnivLE.max : UnivLE.{u, max u v} where
+  Lift α := ULift α
+  up a := ULift.up a
+  down a := ULift.down a
+  up_down := rfl
+  down_up := rfl
+
+class IntoUniv.{v} (α : Type u) where
+  Into : Type v
+  into : α → Shrink
+  back : Shrink → α
+
+structure Equiv (α β) where
+  hom : α → β
+  inv : β → α
+  hom_inv : ∀ {b}, hom (inv b) = b
+  inv_hom : ∀ {a}, inv (hom a) = a
+
+def Equiv.id (α) : Equiv α α :=
+  { hom := _root_.id, inv := _root_.id, hom_inv := rfl, inv_hom := rfl }
